common/Memtype.v
@@ -30,6 +30,7 @@ Require Import Integers.
 Require Import Floats.
 Require Import Values.
 Require Import Memdata.
+Require Import Tags.
 
 (** Memory states are accessed by addresses [b, ofs]: pairs of a block
   identifier [b] and a byte offset [ofs] within that block.
@@ -52,7 +53,11 @@ Inductive permission: Type :=
 | Dead: permission          (* Shadowed by compiler data *)
 .
 
-Module Type MEM.
+Module Type MEM (T:Tag).
+  Module TLib := TagLib T.
+  Import TLib.
+  Module MD := Memdata T.
+  Import MD.
 
 (** The abstract type of memory states. *)
 Parameter mem: Type.
@@ -80,18 +85,12 @@ Parameter free: forall (m: mem) (b: block) (lo hi: Z), option mem.
   addresses [b, ofs] to [b, ofs + size_chunk chunk - 1] in memory state
   [m].  Returns the value read, or [None] if the accessed addresses
   are not readable. *)
-Parameter load: forall (chunk: memory_chunk) (m: mem) (b: block) (ofs: Z), option val.
-Parameter load_vtag: forall (chunk: memory_chunk) (m: mem) (b: block) (ofs: Z), option tag.
+Parameter load: forall (chunk: memory_chunk) (m: mem) (b: block) (ofs: Z), option atom.
 Parameter load_ltags: forall (chunk: memory_chunk) (m: mem) (b: block) (ofs: Z), list tag.
-
-Axiom load_val_has_vtag :
-  forall chunk m b ofs,
-    (exists v, load chunk m b ofs = Some v) <->
-      (exists vt, load_vtag chunk m b ofs = Some vt).
 
 Axiom load_val_has_ltags :
   forall chunk m b ofs,
-    (exists v, load chunk m b ofs = Some v /\ v <> Vundef) <->
+    (exists v, load chunk m b ofs = Some v /\ v <> (Vundef,def_tag)) <->
       (exists lts, load_ltags chunk m b ofs = lts /\ length lts = size_chunk_nat chunk).
 
 (** [store chunk m b ofs v] writes value [v] as memory quantity [chunk]
@@ -103,22 +102,15 @@ Parameter store:
          (m: mem)
          (b: block)
          (ofs: Z)
-         (v: val)
-         (vt: tag)
+         (a: atom)
          (lts: list tag), option mem.
 
 (** [loadv] and [storev] are variants of [load] and [store] where
   the address being accessed is passed as a value (of the [Vptr] kind). *)
 
-Definition loadv (chunk: memory_chunk) (m: mem) (addr: val) : option val :=
+Definition loadv (chunk: memory_chunk) (m: mem) (addr: val) : option atom :=
   match addr with
   | Vptr b ofs => load chunk m b (Ptrofs.unsigned ofs)
-  | _ => None
-  end.
-
-Definition loadv_vtag (chunk: memory_chunk) (m: mem) (addr: val) : option tag :=
-  match addr with
-  | Vptr b ofs => load_vtag chunk m b (Ptrofs.unsigned ofs)
   | _ => None
   end.
 
@@ -128,9 +120,9 @@ Definition loadv_ltags (chunk: memory_chunk) (m: mem) (addr: val) : list tag :=
   | _ => nil
   end.
 
-Definition storev (chunk: memory_chunk) (m: mem) (addr v: val) (vt:tag) (lts: list tag) : option mem :=
+Definition storev (chunk: memory_chunk) (m: mem) (addr: val) (a: atom) (lts: list tag) : option mem :=
   match addr with
-  | Vptr b ofs => store chunk m b (Ptrofs.unsigned ofs) v vt lts
+  | Vptr b ofs => store chunk m b (Ptrofs.unsigned ofs) a lts
   | _ => None
   end.
 
@@ -149,7 +141,6 @@ Parameter storebytes:
          (b: block)
          (ofs: Z)
          (bytes: list memval)
-         (vtag: tag)
          (ltag: list tag), option mem.
 
 (** [free_list] frees all the given (block, lo, hi) triples. *)
@@ -283,20 +274,20 @@ Axiom allowed_access_load:
   accessed: [Vundef], [Vint] or [Vptr] for an integer quantity,
   [Vundef] or [Vfloat] for a float quantity. *)
 Axiom load_type:
-  forall m chunk b ofs v,
-  load chunk m b ofs = Some v ->
+  forall m chunk b ofs v t,
+  load chunk m b ofs = Some (v,t) ->
   Val.has_type v (type_of_chunk chunk).
 
 Axiom load_rettype:
-  forall m chunk b ofs v,
-  load chunk m b ofs = Some v ->
+  forall m chunk b ofs v t,
+  load chunk m b ofs = Some (v,t) ->
   Val.has_rettype v (rettype_of_chunk chunk).
 
 (** For a small integer or float type, the value returned by [load]
   is invariant under the corresponding cast. *)
 Axiom load_cast:
-  forall m chunk b ofs v,
-  load chunk m b ofs = Some v ->
+  forall m chunk b ofs v t,
+  load chunk m b ofs = Some (v,t) ->
   match chunk with
   | Mint8signed => v = Val.sign_ext 8 v
   | Mint8unsigned => v = Val.zero_ext 8 v
@@ -307,11 +298,11 @@ Axiom load_cast:
 
 Axiom load_int8_signed_unsigned:
   forall m b ofs,
-  load Mint8signed m b ofs = option_map (Val.sign_ext 8) (load Mint8unsigned m b ofs).
+  load Mint8signed m b ofs = opt_atom_map (Val.sign_ext 8) (load Mint8unsigned m b ofs).
 
 Axiom load_int16_signed_unsigned:
   forall m b ofs,
-  load Mint16signed m b ofs = option_map (Val.sign_ext 16) (load Mint16unsigned m b ofs).
+  load Mint16signed m b ofs = opt_atom_map (Val.sign_ext 16) (load Mint16unsigned m b ofs).
 
 
 (** ** Properties of [loadbytes]. *)
@@ -378,51 +369,51 @@ Axiom loadbytes_split:
   Moreover, a [store] succeeds if and only if the corresponding access is allowed. *)
 
 Axiom store_valid_block_1:
-  forall chunk m1 b ofs v vt lts m2, store chunk m1 b ofs v vt lts = Some m2 ->
+  forall chunk m1 b ofs v vt lts m2, store chunk m1 b ofs (v,vt) lts = Some m2 ->
   forall ofs', valid_addr m1 ofs' -> valid_addr m2 ofs'.
 Axiom store_valid_block_2:
-  forall chunk m1 b ofs v vt lts m2, store chunk m1 b ofs v vt lts = Some m2 ->
+  forall chunk m1 b ofs v vt lts m2, store chunk m1 b ofs (v,vt) lts = Some m2 ->
   forall b', valid_addr m2 b' -> valid_addr m1 b'.
 
 Axiom perm_store_1:
-  forall chunk m1 b ofs v vt lts m2, store chunk m1 b ofs v vt lts = Some m2 ->
+  forall chunk m1 b ofs v vt lts m2, store chunk m1 b ofs (v,vt) lts = Some m2 ->
   forall b' ofs' p, perm m1 b' ofs' p -> perm m2 b' ofs' p.
 Axiom perm_store_2:
-  forall chunk m1 b ofs v vt lts m2, store chunk m1 b ofs v vt lts = Some m2 ->
+  forall chunk m1 b ofs v vt lts m2, store chunk m1 b ofs (v,vt) lts = Some m2 ->
   forall b' ofs' p, perm m2 b' ofs' p -> perm m1 b' ofs' p.
 
 Axiom allowed_access_store:
   forall m1 chunk b ofs v vt lts,
   allowed_access m1 chunk b ofs ->
-  { m2: mem | store chunk m1 b ofs v vt lts = Some m2 }.
+  { m2: mem | store chunk m1 b ofs (v,vt) lts = Some m2 }.
 Axiom disallowed_access_store:
   forall m1 chunk b ofs v vt lts,
   ~ allowed_access m1 chunk b ofs ->
-  store chunk m1 b ofs v vt lts = None.
+  store chunk m1 b ofs (v,vt) lts = None.
 Axiom store_valid_access_1:
-  forall chunk m1 b ofs v vt lts m2, store chunk m1 b ofs v vt lts = Some m2 ->
+  forall chunk m1 b ofs v vt lts m2, store chunk m1 b ofs (v,vt) lts = Some m2 ->
   forall chunk' b' ofs',
   valid_access m1 chunk' b' ofs' -> valid_access m2 chunk' b' ofs'.
 Axiom store_valid_access_2:
-  forall chunk m1 b ofs v vt lts m2, store chunk m1 b ofs v vt lts = Some m2 ->
+  forall chunk m1 b ofs v vt lts m2, store chunk m1 b ofs (v,vt) lts = Some m2 ->
   forall chunk' b' ofs',
   valid_access m2 chunk' b' ofs' -> valid_access m1 chunk' b' ofs'.
 
 (** Load-store properties. *)
 
 Axiom load_store_similar:
-  forall chunk m1 b ofs v vt lts m2, store chunk m1 b ofs v vt lts = Some m2 ->
+  forall chunk m1 b ofs v vt lts m2, store chunk m1 b ofs (v,vt) lts = Some m2 ->
   forall chunk',
   size_chunk chunk' = size_chunk chunk ->
   align_chunk chunk' <= align_chunk chunk ->
-  exists v', load chunk' m2 b ofs = Some v' /\ decode_encode_val v chunk chunk' v'.
+  exists v' t, load chunk' m2 b ofs = Some (v',t) /\ decode_encode_val v chunk chunk' v'.
 
 Axiom load_store_same:
-  forall chunk m1 b ofs v vt lts m2, store chunk m1 b ofs v vt lts = Some m2 ->
-  load chunk m2 b ofs = Some (Val.load_result chunk v).
+  forall chunk m1 b ofs v vt lts m2, store chunk m1 b ofs (v,vt) lts = Some m2 ->
+  load chunk m2 b ofs = Some (Val.load_result chunk v, vt).
 
 Axiom load_store_other:
-  forall chunk m1 b ofs v vt lts m2, store chunk m1 b ofs v vt lts = Some m2 ->
+  forall chunk m1 b ofs v vt lts m2, store chunk m1 b ofs (v,vt) lts = Some m2 ->
   forall chunk' b' ofs',
   b' <> b
   \/ ofs' + size_chunk chunk' <= ofs
@@ -440,32 +431,32 @@ Definition compat_pointer_chunks (chunk1 chunk2: memory_chunk) : Prop :=
 
 Axiom load_store_pointer_overlap:
   forall chunk m1 b ofs v_b v_o m2 chunk' ofs' v vt lts,
-  store chunk m1 b ofs (Vptr v_b v_o) vt lts = Some m2 ->
+  store chunk m1 b ofs (Vptr v_b v_o, vt) lts = Some m2 ->
   load chunk' m2 b ofs' = Some v ->
   ofs' <> ofs ->
   ofs' + size_chunk chunk' > ofs ->
   ofs + size_chunk chunk > ofs' ->
-  v = Vundef.
+  v = (Vundef, def_tag).
 Axiom load_store_pointer_mismatch:
   forall chunk m1 b ofs v_b v_o m2 chunk' v vt lts,
-  store chunk m1 b ofs (Vptr v_b v_o) vt lts = Some m2 ->
+  store chunk m1 b ofs (Vptr v_b v_o, vt) lts = Some m2 ->
   load chunk' m2 b ofs = Some v ->
   ~compat_pointer_chunks chunk chunk' ->
-  v = Vundef.
+  v = (Vundef, def_tag).
 Axiom load_pointer_store:
-  forall chunk m1 b ofs v vt lts m2 chunk' b' ofs' v_b v_o,
-  store chunk m1 b ofs v vt lts = Some m2 ->
-  load chunk' m2 b' ofs' = Some(Vptr v_b v_o) ->
+  forall chunk m1 b ofs v vt lts m2 chunk' b' ofs' v_b v_o vt',
+  store chunk m1 b ofs (v,vt) lts = Some m2 ->
+  load chunk' m2 b' ofs' = Some(Vptr v_b v_o, vt') ->
   (v = Vptr v_b v_o /\ compat_pointer_chunks chunk chunk' /\ b' = b /\ ofs' = ofs)
   \/ (b' <> b \/ ofs' + size_chunk chunk' <= ofs \/ ofs + size_chunk chunk <= ofs').
 
 (** Load-store properties for [loadbytes]. *)
 
 Axiom loadbytes_store_same:
-  forall chunk m1 b ofs v vt lts m2, store chunk m1 b ofs v vt lts = Some m2 ->
-  loadbytes m2 b ofs (size_chunk chunk) = Some(encode_val chunk v).
+  forall chunk m1 b ofs v vt lts m2, store chunk m1 b ofs (v,vt) lts = Some m2 ->
+  loadbytes m2 b ofs (size_chunk chunk) = Some(encode_val chunk (v,vt)).
 Axiom loadbytes_store_other:
-  forall chunk m1 b ofs v vt lts m2, store chunk m1 b ofs v vt lts = Some m2 ->
+  forall chunk m1 b ofs v vt lts m2, store chunk m1 b ofs (v,vt) lts = Some m2 ->
   forall b' ofs' n,
   b' <> b \/ n <= 0 \/ ofs' + n <= ofs \/ ofs + size_chunk chunk <= ofs' ->
   loadbytes m2 b' ofs' n = loadbytes m1 b' ofs' n.
@@ -475,26 +466,26 @@ Axiom loadbytes_store_other:
 
 Axiom store_signed_unsigned_8:
   forall m b ofs v vt lts,
-  store Mint8signed m b ofs v vt lts = store Mint8unsigned m b ofs v vt lts.
+  store Mint8signed m b ofs (v,vt) lts = store Mint8unsigned m b ofs (v,vt) lts.
 Axiom store_signed_unsigned_16:
   forall m b ofs v vt lts,
-  store Mint16signed m b ofs v vt lts = store Mint16unsigned m b ofs v vt lts.
+  store Mint16signed m b ofs (v,vt) lts = store Mint16unsigned m b ofs (v,vt) lts.
 Axiom store_int8_zero_ext:
   forall m b ofs n vt lts,
-  store Mint8unsigned m b ofs (Vint (Int.zero_ext 8 n)) vt lts =
-  store Mint8unsigned m b ofs (Vint n) vt lts.
+  store Mint8unsigned m b ofs (Vint (Int.zero_ext 8 n), vt) lts =
+  store Mint8unsigned m b ofs (Vint n, vt) lts.
 Axiom store_int8_sign_ext:
   forall m b ofs n vt lts,
-  store Mint8signed m b ofs (Vint (Int.sign_ext 8 n)) vt lts =
-  store Mint8signed m b ofs (Vint n) vt lts.
+  store Mint8signed m b ofs (Vint (Int.sign_ext 8 n), vt) lts =
+  store Mint8signed m b ofs (Vint n, vt) lts.
 Axiom store_int16_zero_ext:
   forall m b ofs n vt lts,
-  store Mint16unsigned m b ofs (Vint (Int.zero_ext 16 n)) vt lts =
-  store Mint16unsigned m b ofs (Vint n) vt lts.
+  store Mint16unsigned m b ofs (Vint (Int.zero_ext 16 n), vt) lts =
+  store Mint16unsigned m b ofs (Vint n, vt) lts.
 Axiom store_int16_sign_ext:
   forall m b ofs n vt lts,
-  store Mint16signed m b ofs (Vint (Int.sign_ext 16 n)) vt lts =
-  store Mint16signed m b ofs (Vint n) vt lts.
+  store Mint16signed m b ofs (Vint (Int.sign_ext 16 n), vt) lts =
+  store Mint16signed m b ofs (Vint n, vt) lts.
 
 (** ** Properties of [storebytes]. *)
 
@@ -503,49 +494,49 @@ Axiom store_int16_sign_ext:
   on the addressed memory area. *)
 
 Axiom perm_storebytes_1:
-  forall m1 b ofs bytes vt ltags m2, storebytes m1 b ofs bytes vt ltags = Some m2 ->
+  forall m1 b ofs bytes ltags m2, storebytes m1 b ofs bytes ltags = Some m2 ->
   forall b' ofs' p, perm m1 b' ofs' p -> perm m2 b' ofs' p.
 Axiom perm_storebytes_2:
-  forall m1 b ofs bytes vt ltags m2, storebytes m1 b ofs bytes vt ltags = Some m2 ->
+  forall m1 b ofs bytes ltags m2, storebytes m1 b ofs bytes ltags = Some m2 ->
   forall b' ofs' p, perm m2 b' ofs' p -> perm m1 b' ofs' p.
 Axiom storebytes_valid_access_1:
-  forall m1 b ofs bytes vt ltags m2, storebytes m1 b ofs bytes vt ltags = Some m2 ->
+  forall m1 b ofs bytes ltags m2, storebytes m1 b ofs bytes ltags = Some m2 ->
   forall chunk' b' ofs',
   valid_access m1 chunk' b' ofs' -> valid_access m2 chunk' b' ofs'.
 Axiom storebytes_valid_access_2:
-  forall m1 b ofs bytes vt ltags m2, storebytes m1 b ofs bytes vt ltags = Some m2 ->
+  forall m1 b ofs bytes ltags m2, storebytes m1 b ofs bytes ltags = Some m2 ->
   forall chunk' b' ofs',
   valid_access m2 chunk' b' ofs' -> valid_access m1 chunk' b' ofs'.
 Axiom storebytes_allowed_access_1:
-  forall m1 b ofs bytes vt ltags m2, storebytes m1 b ofs bytes vt ltags = Some m2 ->
+  forall m1 b ofs bytes ltags m2, storebytes m1 b ofs bytes ltags = Some m2 ->
   forall chunk' b' ofs',
   allowed_access m1 chunk' b' ofs' -> allowed_access m2 chunk' b' ofs'.
 Axiom storebytes_allowed_access_2:
-  forall m1 b ofs bytes vt ltags m2, storebytes m1 b ofs bytes vt ltags = Some m2 ->
+  forall m1 b ofs bytes ltags m2, storebytes m1 b ofs bytes ltags = Some m2 ->
   forall chunk' b' ofs',
   allowed_access m2 chunk' b' ofs' -> allowed_access m1 chunk' b' ofs'.
 Axiom storebytes_valid_block_1:
-  forall m1 b ofs bytes vt ltags m2, storebytes m1 b ofs bytes vt ltags = Some m2 ->
+  forall m1 b ofs bytes ltags m2, storebytes m1 b ofs bytes ltags = Some m2 ->
   forall ofs', valid_addr m1 ofs' -> valid_addr m2 ofs'.
 Axiom storebytes_valid_block_2:
-  forall m1 b ofs bytes vt ltags m2, storebytes m1 b ofs bytes vt ltags = Some m2 ->
+  forall m1 b ofs bytes ltags m2, storebytes m1 b ofs bytes ltags = Some m2 ->
   forall ofs', valid_addr m2 ofs' -> valid_addr m1 ofs'.
 
 (** Connections between [store] and [storebytes]. *)
 
 Axiom storebytes_store:
   forall m1 b ofs chunk v vt lts m2,
-  storebytes m1 b ofs (encode_val chunk v) vt lts = Some m2 ->
+  storebytes m1 b ofs (encode_val chunk (v,vt)) lts = Some m2 ->
   (align_chunk chunk | ofs) ->
-  store chunk m1 b ofs v vt lts = Some m2.
+  store chunk m1 b ofs (v,vt) lts = Some m2.
 
 (** Load-store properties. *)
 
 Axiom loadbytes_storebytes_same:
-  forall m1 b ofs bytes vt lts m2, storebytes m1 b ofs bytes vt lts = Some m2 ->
+  forall m1 b ofs bytes lts m2, storebytes m1 b ofs bytes lts = Some m2 ->
   loadbytes m2 b ofs (Z.of_nat (length bytes)) = Some bytes.
 Axiom loadbytes_storebytes_other:
-  forall m1 b ofs bytes vt lts m2, storebytes m1 b ofs bytes vt lts = Some m2 ->
+  forall m1 b ofs bytes lts m2, storebytes m1 b ofs bytes lts = Some m2 ->
   forall b' ofs' len,
   len >= 0 ->
   b' <> b
@@ -553,7 +544,7 @@ Axiom loadbytes_storebytes_other:
   \/ ofs + Z.of_nat (length bytes) <= ofs' ->
   loadbytes m2 b' ofs' len = loadbytes m1 b' ofs' len.
 Axiom load_storebytes_other:
-  forall m1 b ofs bytes vt lts m2, storebytes m1 b ofs bytes vt lts = Some m2 ->
+  forall m1 b ofs bytes lts m2, storebytes m1 b ofs bytes lts = Some m2 ->
   forall chunk b' ofs',
   b' <> b
   \/ ofs' + size_chunk chunk <= ofs
@@ -563,16 +554,16 @@ Axiom load_storebytes_other:
 (** Composing or decomposing [storebytes] operations at adjacent addresses. *)
 
 Axiom storebytes_concat:
-  forall m b ofs bytes1 vt lts1 m1 bytes2 lts2 m2,
-  storebytes m b ofs bytes1 vt lts1 = Some m1 ->
-  storebytes m1 b (ofs + Z.of_nat(length bytes1)) bytes2 vt lts2 = Some m2 ->
-  storebytes m b ofs (bytes1 ++ bytes2) vt (lts1 ++ lts2) = Some m2.
+  forall m b ofs bytes1 lts1 m1 bytes2 lts2 m2,
+  storebytes m b ofs bytes1 lts1 = Some m1 ->
+  storebytes m1 b (ofs + Z.of_nat(length bytes1)) bytes2 lts2 = Some m2 ->
+  storebytes m b ofs (bytes1 ++ bytes2) (lts1 ++ lts2) = Some m2.
 Axiom storebytes_split:
-  forall m b ofs bytes1 bytes2 vt lts1 lts2 m2,
-  storebytes m b ofs (bytes1 ++ bytes2) vt (lts1 ++ lts2) = Some m2 ->
+  forall m b ofs bytes1 bytes2 lts1 lts2 m2,
+  storebytes m b ofs (bytes1 ++ bytes2) (lts1 ++ lts2) = Some m2 ->
   exists m1,
-     storebytes m b ofs bytes1 vt lts1 = Some m1
-  /\ storebytes m1 b (ofs + Z.of_nat(length bytes1)) bytes2 vt lts2 = Some m2.
+     storebytes m b ofs bytes1 lts1 = Some m1
+  /\ storebytes m1 b (ofs + Z.of_nat(length bytes1)) bytes2 lts2 = Some m2.
 
 (** ** Properties of [alloc]. *)
 
