common/Tags.v
@@ -1,0 +1,43 @@
+Require Import Coqlib.
+Require Import AST.
+Require Import Integers.
+Require Import Floats.
+Require Import Values.
+
+Module Type Tag.
+
+(** For now we will just stick the tag type in a parameter here. *)
+  Parameter tag : Type.
+  Parameter tag_eq_dec : forall (t1 t2:tag), {t1 = t2} + {t1 <> t2}.
+  Parameter def_tag : tag.
+
+End Tag.
+
+Module TagLib (T:Tag).
+  Export T.
+
+  Definition atom : Type := val * tag.
+  Definition atom_map (f:val -> val) (a:atom) :=
+    let '(v,t) := a in (f v, t).
+  Definition at_map (f:val -> val) (a:atom*tag) :=
+    let '(v,t,t') := a in (f v, t, t').
+
+  Definition opt_atom_map (f:val -> val) (a:option atom) :=
+    option_map (atom_map f) a.
+
+  Definition opt_at_map (f:val -> val) (a:option (atom*tag)) :=
+    option_map (at_map f) a.
+
+  Lemma atom_eq_dec :
+    forall (a1 a2:atom),
+      {a1 = a2} + {a1 <> a2}.
+  Proof.
+    repeat decide equality.
+    apply tag_eq_dec.
+    apply Int.eq_dec.
+    apply Int64.eq_dec.
+    apply Float.eq_dec.
+    apply Float32.eq_dec.
+    apply Ptrofs.eq_dec.
+  Qed.  
+End TagLib.
